semantics/semanticPrimitivesScript.sml
@@ -1135,12 +1135,13 @@ Definition do_app_def:
             else NONE
         | _ => NONE
       )
-    | (Aw8setBit_unsafe b, [Loc _ lnum; Litv (IntLit i)]) =>
+    | (Aw8updateBit_unsafe, [Loc _ lnum; Litv (IntLit i); v]) =>
         (case store_lookup lnum s of
           SOME (W8array ws) =>
-            if 0 ≤ i ∧ i < 8 * &LENGTH ws then
+            if 0 ≤ i ∧ i < 8 * &LENGTH ws ∧ (v = Boolv T ∨ v = Boolv F) then
               (case store_assign lnum
-                      (W8array (LUPDATE (((Num i MOD 8) :+ b) (EL (Num i DIV 8) ws))
+                      (W8array (LUPDATE (((Num i MOD 8) :+ (v = Boolv T))
+                                         (EL (Num i DIV 8) ws))
                                         (Num i DIV 8) ws)) s of
                   NONE => NONE
                 | SOME s' => SOME ((s',t), Rval (Conv NONE []))
