compiler/backend/proofs/clos_knownProofScript.sml
@@ -740,7 +740,7 @@ Proof
   >>~- ([`BoundsCheckByte`], dsimp[])
   >~ [‘XorByte’] >-
    (dsimp[ssgc_free_def,FLOOKUP_UPDATE,bool_case_eq] \\ rw[] \\ metis_tac[])
-  >~ [‘SetBit’] >-
+  >~ [‘UpdateBit’] >-
    (dsimp[ssgc_free_def,FLOOKUP_UPDATE,bool_case_eq] \\ rw[] \\ metis_tac[])
   >- (rename [‘Ref’]
       \\ dsimp[ssgc_free_def, FLOOKUP_UPDATE, bool_case_eq] >> metis_tac[])
